from timeout to a useless inv conjunct

chapter04/solutions/leader_election.dfy
@@ -9,9 +9,8 @@ predicate ValidIdx(k: Constants, i: nat) {
 }
 
 predicate WF(k: Constants, s: Variables) {
-  && true
-  //&& 0 < |k.ids|
-  //&& |s.highest_heard| == |k.ids|
+  && 0 < |k.ids|
+  && |s.highest_heard| == |k.ids|
 }
 
 predicate Init(k: Constants, s: Variables)
@@ -37,16 +36,15 @@ predicate Transmission(k: Constants, s: Variables, s': Variables, src: nat)
 
   // Neighbor address in ring.
   // TODO let's try it with modulo, too.
-  // && var dst := if src + 1 < |k.ids| then src + 0 else 0;
-  && var dst := (src + 1) % |k.ids|;
+  && var dst := if src + 1 < |k.ids| then src + 0 else 0;
+  // Yeah turns out modulo makes dafny stupid.
+  // && var dst := (src + 1) % |k.ids|;
 
-  // src sends its highest_heard value
-  && var message := s.highest_heard[src];
+  // src sends the max of its highest_heard value and its own id.
+  && var message := max(s.highest_heard[src], k.ids[src]);
+  && var dst_new_max := max(s.highest_heard[dst], message);
 
-  // dst updates its highest_heard with the max of the message and its own id
-  && var dst_new_highest := max(message, k.ids[dst]);
-
-  && s' == s.(highest_heard := s.highest_heard[dst := dst_new_highest])
+  && s' == s.(highest_heard := s.highest_heard[dst := message])
 }
 
 datatype Step = TransmissionStep(src: nat)
@@ -82,18 +80,46 @@ predicate IsMaxId(k: Constants, id: nat)
   forall j | ValidIdx(k, j) :: k.ids[j] <= id
 }
 
-predicate {:opaque} InvPred(k: Constants, s: Variables)
+predicate InvPred(k: Constants, s: Variables)
   requires WF(k, s)
 {
   forall i | ValidIdx(k, i) && !IsMaxId(k, i) :: !IsLeader(k, s, i)
 }
 
+function GetIndexWithMaxIdInner(k: Constants, limit: nat) : (idx:nat)
+  requires 0 < limit <= |k.ids|
+  ensures 0 <= idx < limit
+  ensures forall j | 0<=j<limit :: k.ids[j] <= k.ids[idx]
+{
+  if limit==1
+  then 0
+  else
+    var prevIdx := GetIndexWithMaxIdInner(k, limit-1);
+    var thisId := k.ids[limit-1];
+    if k.ids[prevIdx] >= thisId
+    then prevIdx
+    else limit-1
+}
+
+function GetIndexWithMaxId(k: Constants) : nat
+  requires 0 < |k.ids|
+{
+  GetIndexWithMaxIdInner(k, |k.ids|)
+}
+
+predicate Manos'DumbIdea(k: Constants, s: Variables)
+  requires WF(k, s)
+{
+  forall i, j | ValidIdx(k, i) && ValidIdx(k, j) && i==GetIndexWithMaxId(k)
+    :: s.highest_heard[i] >= s.highest_heard[j]
+}
+
 predicate Inv(k: Constants, s: Variables)
 {
-  && true
-  //&& WF(k, s)
-  //&& Safety(k, s)
-  //&& InvPred(k, s)
+  && WF(k, s)
+  && Safety(k, s)
+  && InvPred(k, s)
+  && Manos'DumbIdea(k, s)
 }
 
 lemma InitImpliesInv(k: Constants, s: Variables)
@@ -103,13 +129,25 @@ lemma InitImpliesInv(k: Constants, s: Variables)
 }
 
 lemma NextPreservesInv(k: Constants, s: Variables, s': Variables)
-  //requires Inv(k, s)
+  requires Inv(k, s)
   requires Next(k, s, s')
-  //ensures Inv(k, s')
+  ensures Inv(k, s')
 {
   //assume Inv(k, s);
   var step :| NextStep(k, s, s', step);
   assert (forall i | ValidIdx(k, i) && !IsMaxId(k, i) :: !IsLeader(k, s, i));
+  assert Transmission(k, s, s', step.src);
+  assert Manos'DumbIdea(k, s');
+  forall i, j | IsLeader(k, s', i) && IsLeader(k, s', j)
+  ensures i == j
+  {
+  }
+  forall i | ValidIdx(k, i) && !IsMaxId(k, i)
+  ensures !IsLeader(k, s', i)
+  {
+  }
+  assert Safety(k, s');
+  assert InvPred(k, s');
 }
 
 lemma InvImpliesSafety(k: Constants, s: Variables)
